theories/Libs/CookPrelim/PolyBounds.v
@@ -23,18 +23,7 @@ Proof.
   induction l; cbn -[Nat.add Nat.mul]. 
   - lia.
   - unfold concat_time in IHl. rewrite IHl. lia. 
-Qed. 
-
-Tactic Notation "poly_mono" constr(H) "at" ne_integer_list(occ) :=
-  let He := fresh in specialize H as He; match type of He with
-                    | _ /\ monotonic _ => unfold monotonic in He; setoid_rewrite (proj2 He) at occ
-                    | monotonic _ /\ _ => unfold monotonic in He; setoid_rewrite (proj1 He) at occ
-                    end; clear He. 
-Tactic Notation "poly_mono" constr(H) :=
-  let He := fresh in specialize H as He; match type of He with
-                    | _ /\ monotonic _ => unfold monotonic in He; erewrite (proj2 He)
-                    | monotonic _ /\ _ => unfold monotonic in He; erewrite (proj1 He)
-                    end; clear He.
+Qed.
 
 Definition c__moduloBound :=  c__divmod + c__modulo + c__sub.
 Lemma modulo_time_bound x y: 
@@ -70,25 +59,28 @@ Section fixXEq.
       rewrite Nat.le_min_l. unfold poly__listInDecb. 
       rewrite list_size_cons. unfold c__listsizeCons; leq_crossout.
   Qed.
-  Lemma list_in_decb_poly : monotonic poly__listInDecb /\ inOPoly poly__listInDecb. 
-  Proof. 
-    unfold poly__listInDecb; split; smpl_inO. 
-  Qed. 
+
+  Lemma list_in_decb_poly: inOPoly poly__listInDecb.
+  Proof. unfold poly__listInDecb. smpl_inO. Qed.
+  #[export] Instance list_in_decb_mono: Proper (le ==> le) poly__listInDecb.
+  Proof. unfold poly__listInDecb. solve_proper. Qed.
 
   Definition poly__listInclDecb n := n * poly__listInDecb n + (n + 1) * c__list_incl_decb.
   Lemma list_incl_decb_time_bound (l1 l2 :list X) : list_incl_decb_time l1 l2 <= poly__listInclDecb (size (enc l1) + size (enc l2)). 
   Proof.
     induction l1; cbn. 
     - unfold poly__listInclDecb. nia. 
-    - rewrite list_in_decb_time_bound. rewrite IHl1. 
-      poly_mono list_in_decb_poly. 2: { instantiate (1 := size (enc (a :: l1)) + size (enc l2)). lia. }
-      unfold poly__listInclDecb. rewrite list_size_cons at 2 4. 
-      poly_mono list_in_decb_poly at 2. 2 : { instantiate (1 := size (enc (a :: l1)) + size (enc l2)). rewrite list_size_cons. lia. }
-      unfold c__listsizeCons. nia. 
-  Qed. 
-  Lemma list_incl_decb_poly : monotonic poly__listInclDecb /\ inOPoly poly__listInclDecb.
-  Proof. 
-    unfold poly__listInclDecb; split; smpl_inO; apply list_in_decb_poly. 
+    - rewrite list_in_decb_time_bound. rewrite IHl1.
+      setoid_replace (size (enc l2)) with (size (enc (a :: l1)) + size (enc l2)) using relation le at 1 by easy.
+      unfold poly__listInclDecb. rewrite list_size_cons at 2 4.
+      setoid_replace ((size (enc l1) + size (enc l2))) with (size (enc (a :: l1)) + size (enc l2)) using relation le at 2.
+      + unfold c__listsizeCons. nia.
+      + rewrite list_size_cons. lia.
+  Qed.
+
+  Lemma list_incl_decb_poly : inOPoly poly__listInclDecb.
+  Proof.
+    unfold poly__listInclDecb; smpl_inO; apply list_in_decb_poly. 
   Qed. 
 
   Definition poly__dupfreeb n := n * poly__listInDecb n + (n + 1) * c__dupfreeb. 
@@ -96,17 +88,19 @@ Section fixXEq.
   Proof. 
     induction l; cbn. 
     - unfold poly__dupfreeb; nia. 
-    - rewrite list_in_decb_time_bound. rewrite IHl. 
-      poly_mono list_in_decb_poly. 2: { instantiate (1 := size (enc (a :: l))). rewrite list_size_cons. nia. }
-      unfold poly__dupfreeb. 
-      poly_mono list_in_decb_poly at 2. 2: { instantiate (1 := size (enc (a :: l))). rewrite list_size_cons. nia. }
-      rewrite list_size_cons at 3 5. unfold c__listsizeCons. nia. 
-  Qed. 
-  Lemma dupfreeb_poly : monotonic poly__dupfreeb /\ inOPoly poly__dupfreeb. 
+    - rewrite list_in_decb_time_bound. rewrite IHl.
+      unfold poly__dupfreeb.
+      setoid_replace (size (enc l)) with (size (enc (a :: l))) using relation le at 1 3 by now rewrite list_size_cons.
+      rewrite list_size_cons at 3 5. unfold c__listsizeCons. nia.
+  Qed.
+
+  Lemma dupfreeb_poly : inOPoly poly__dupfreeb. 
   Proof. 
-    unfold poly__dupfreeb; split; smpl_inO; apply list_in_decb_poly. 
-  Qed. 
-End fixXEq. 
+    unfold poly__dupfreeb; smpl_inO; apply list_in_decb_poly. 
+  Qed.
+  #[export] Instance dupfreeb_mono: Proper (le ==> le) poly__dupfreeb.
+  Proof. unfold poly__dupfreeb. solve_proper. Qed.
+End fixXEq.
 
 Section fixX.
   Context {X : Type}.
@@ -118,15 +112,16 @@ Section fixX.
   Context {RY : encodable Y}.
 
   Lemma forallb_time_bound_env (predT : Y -> X -> nat) (f : nat -> nat):
-    (forall (a : X) (y : Y), predT y a <= f (size(enc a) + size(enc y))) /\ monotonic f 
+    (forall (a : X) (y : Y), predT y a <= f (size(enc a) + size(enc y))) /\ Proper (le ==> le) f 
     -> forall (l : list X) (y : Y), forallb_time (predT y) l <= (|l| +1) * (f(size (enc l) + size(enc y)) + c__forallb). 
   Proof. 
     intros [H1 H2]. intros. induction l. 
     - cbn. lia.   
-    - cbn. rewrite <- Nat.add_assoc, IHl, H1. unfold monotonic in H2. 
-      rewrite H2 with (x' := size (enc (a :: l)) + size(enc y)). 2: rewrite list_size_cons; nia. 
-      setoid_rewrite H2 with (x' := size(enc (a::l)) + size(enc y)) at 2. 2: rewrite list_size_cons; nia. 
-      nia.
+    - cbn. rewrite <- Nat.add_assoc, IHl, H1.
+      setoid_replace (size (enc a) + size (enc y)) with (size (enc (a :: l)) + size(enc y)) using relation le.
+      setoid_replace (size (enc l) + size (enc y)) with (size(enc (a::l)) + size(enc y)) using relation le.
+      reflexivity.
+      all: rewrite list_size_cons; nia.
   Qed. 
 
   Lemma nth_error_time_bound : 
@@ -136,16 +131,16 @@ Section fixX.
   Qed. 
 
   Lemma map_time_bound_env (fT : Y -> X -> nat) (f__bound : nat -> nat): 
-    (forall (env : Y) (ele : X), fT env ele <= f__bound (size (enc env) + size (enc ele))) /\ monotonic f__bound
+    (forall (env : Y) (ele : X), fT env ele <= f__bound (size (enc env) + size (enc ele))) /\ Proper (le ==> le) f__bound
     -> forall (env : Y) (l : list X), map_time (fT env) l <= (|l| + 1) * (f__bound (size (enc env) + size (enc l)) + 1) * (c__map + 1). 
   Proof. 
     intros [H1 H2] env l. induction l; cbn -[c__map]. 
     - nia. 
-    - rewrite IHl. rewrite H1. unfold monotonic in H2. 
+    - rewrite IHl. rewrite H1. 
       rewrite H2 at 1. 2: (replace_le (size (enc a)) with (size (enc (a::l))) by (rewrite list_size_cons; lia)); reflexivity. 
       setoid_rewrite H2 at 2. 2: (replace_le (size (enc l)) with (size (enc (a::l))) by (rewrite list_size_cons; lia)); reflexivity. 
-      nia. 
-  Qed. 
+      nia.
+  Qed.
 
   Definition poly__concat n := (n + 1) * c__concat.
   Lemma concat_time_bound (l : list (list X)) : concat_time l <= poly__concat (size (enc l)). 
@@ -153,11 +148,12 @@ Section fixX.
     unfold concat_time. induction l; cbn -[Nat.add Nat.mul].
     - unfold poly__concat. nia. 
     - rewrite IHl. unfold poly__concat. rewrite list_size_cons. rewrite list_size_length. unfold c__concat, c__listsizeCons; nia.
-  Qed. 
-  Lemma concat_poly : monotonic poly__concat /\ inOPoly poly__concat. 
-  Proof. 
-    split; unfold poly__concat; smpl_inO. 
-  Qed. 
+  Qed.
+ 
+  Lemma concat_poly : inOPoly poly__concat. 
+  Proof. unfold poly__concat; smpl_inO. Qed.
+  #[export] Instance concat_mono: Proper (le ==> le) poly__concat.
+  Proof. unfold poly__concat. solve_proper. Qed. 
 End fixX.
 
 Section fixXY.
@@ -167,8 +163,8 @@ Section fixXY.
   Context {H1 : encodable Z}.
 
   Lemma fold_right_time_bound_env (step : Z -> Y -> X -> X) (stepT : Z -> Y -> X -> nat) (f__arg f__size : nat -> nat): 
-    (forall (acc : X) (ele : Y) (env : Z), stepT env ele acc <= f__arg (size (enc acc) + size (enc ele) + size (enc env))) /\ monotonic f__arg
-    -> (forall (acc : X) (ele : Y) (env : Z), size (enc (step env ele acc)) <= size (enc acc) + f__size (size (enc ele) + size (enc env))) /\ monotonic f__size
+    (forall (acc : X) (ele : Y) (env : Z), stepT env ele acc <= f__arg (size (enc acc) + size (enc ele) + size (enc env))) /\ Proper (le ==> le) f__arg
+    -> (forall (acc : X) (ele : Y) (env : Z), size (enc (step env ele acc)) <= size (enc acc) + f__size (size (enc ele) + size (enc env))) /\ Proper (le ==> le) f__size
     -> forall (l : list Y) (acc : X) (env : Z), fold_right_time (step env) (stepT env) l acc <= (|l| + 1) * f__arg (|l| * f__size (size(enc l) + size (enc env)) + size (enc acc) + size(enc l) + size (enc env)) + (|l| + 1) * c__fold_right. 
   Proof. 
     intros [G1 G2] [F1 F2] l init env. 
@@ -178,7 +174,7 @@ Section fixXY.
       intros l' l''. revert l'. induction l''; intros.
       - cbn. lia. 
       - cbn. rewrite F1. rewrite IHl''. 2: { now rewrite app_comm_cons' in H2. } 
-        unfold monotonic in F2. setoid_rewrite F2 at 2. 
+        setoid_rewrite F2 at 2. 
         2: (replace_le (size(enc a)) with (size (enc (a::l''))) by (apply list_el_size_bound; eauto)); reflexivity. 
         rewrite F2 at 1. 2: (replace_le (size (enc l'')) with (size (enc (a::l''))) by (rewrite list_size_cons; lia)); reflexivity. 
         nia. 
@@ -189,7 +185,7 @@ Section fixXY.
     - cbn -[c__fold_right]. rewrite IHl. clear IHl.
       2: { intros. specialize (H3 (a::l') l''). apply H3. rewrite H2. eauto. } 
       rewrite G1. 
-      unfold monotonic in *. erewrite G2. 
+      erewrite G2. 
       2: { rewrite H3. 2: assert (a::l = [a] ++l) as -> by eauto; easy.
            erewrite F2. 2: (replace_le (size (enc l)) with (size (enc (a::l))) by (rewrite list_size_cons; lia)); reflexivity. 
            replace_le (size (enc a)) with (size (enc (a::l))) by (rewrite list_size_cons; lia). 
@@ -216,8 +212,8 @@ Section prodLists_bound.
     unfold prodLists_time. rewrite !list_size_length. 
     unfold poly__prodLists. solverec. 
   Qed. 
-  Lemma prodLists_poly : monotonic poly__prodLists /\ inOPoly poly__prodLists. 
-  Proof. 
-    unfold poly__prodLists; split; smpl_inO. 
-  Qed. 
+  Lemma prodLists_poly : inOPoly poly__prodLists.
+  Proof. unfold poly__prodLists; smpl_inO. Qed.
+  #[export] Instance prodLists_mono: Proper (le ==> le) poly__prodLists.
+  Proof. unfold poly__prodLists. solve_proper. Qed.
 End prodLists_bound. 
